one function in DPE init_engine_context with a tagged union

test/engine/DPE.c
@@ -1,0 +1,99 @@
+#include <stdlib.h>
+#include <stdint.h>
+#include <stdbool.h>
+#include "../include/PulseMacros.h"
+#include "DPE.h"
+
+INCLUDE (
+module U8 = FStar.UInt8
+
+noeq
+type context_payload_spec =
+| PL_Engine : uds:Seq.seq U8.t -> context_payload_spec
+| PL_L0     : cdi:Seq.seq U8.t -> context_payload_spec
+| PL_L1 //TBD
+
+
+let owns_payload (c: u_context_t_spec) (s: context_payload_spec) (f:bool) : slprop =
+  match c with
+  | Case_u_context_t_uds uds ->
+    exists* v. 
+      (uds |-> v) **
+      maybe f (freeable_array uds) **
+      pure (s == PL_Engine v)
+  | Case_u_context_t_cdi cdi ->
+    exists* v.
+      (cdi |-> v) **
+      maybe f (freeable_array cdi) **
+      pure (s == PL_L0 v)
+  | Case_u_context_t_l1_context l1 ->
+    pure (s == PL_L1)
+
+[@@ pulse_unfold]
+let tag_relation (s:context_t_spec): slprop =
+  pure (match s.tag with
+        | 0uy -> Case_u_context_t_uds? s.payload
+        | 1uy -> Case_u_context_t_cdi? s.payload
+        | 2uy -> Case_u_context_t_l1_context? s.payload
+        | _ -> False)
+
+[@@ pulse_unfold]
+let owns_context_t_aux (u: ref context_t) (pl: context_payload_spec) (f:bool) (s:context_t_spec) : slprop =
+    context_t_pred u s **
+    owns_payload s.payload pl f **
+    tag_relation s
+
+[@@ pulse_unfold]
+let is_context (u: ref context_t) (pl: context_payload_spec) (f:bool) : slprop =
+  exists* s. owns_context_t_aux u pl f s
+
+ghost
+fn intro_owns_payload_a (a:u_context_t_spec { Case_u_context_t_uds? a }) (#f:bool) (#v:_) 
+requires (Case_u_context_t_uds?._0 a |-> v) ** maybe f (freeable_array (Case_u_context_t_uds?._0 a))
+ensures owns_payload (Case_u_context_t_uds (Case_u_context_t_uds?._0 a)) (PL_Engine v) f
+{
+  fold owns_payload (Case_u_context_t_uds (Case_u_context_t_uds?._0 a)) (PL_Engine v) f
+}
+
+ghost
+fn intro_owns_payload
+    (u:ref context_t)
+    (#s:context_t_spec)
+    (#pl:u_context_t_spec)
+    (#ib:context_payload_spec) #f
+requires
+    context_t_pred u s **
+    owns_payload pl ib f **
+    pure (s.payload == pl) **
+    tag_relation s
+ensures is_context u ib f
+{
+  rewrite each pl as s.payload;
+}
+)
+
+ERASED_ARG(#uds_bytes:erased (Seq.seq UInt8.t))
+ERASED_ARG(#p:_)
+PRESERVES(uds |-> Frac p uds_bytes)
+RETURNS(c:ref context_t)
+ENSURES(exists* s. is_context c s _true_ ** freeable c ** pure (PL_Engine? s))
+context_t* init_engine_context(ISARRAY(UDS_LEN) uint8_t *uds)
+{
+  ISARRAY(UDS_LEN) uint8_t *uds_buf = (uint8_t*)malloc(sizeof(uint8_t)*UDS_LEN);
+  LEMMA(intro_maybe (freeable_array (!uds_buf)));
+  context_t *ctx = (context_t*)malloc(sizeof(context_t));
+  LEMMA(
+    context_t_explode (!ctx);
+    u_context_t_change_uds (! (!ctx)).payload;
+    u_context_t_explode (! (!ctx)).payload
+  );
+  ctx->tag = ENGINE_CONTEXT;
+  ctx->payload.uds = uds_buf;
+  LEMMA(
+    intro_owns_payload_a (Case_u_context_t_uds (!uds_buf));
+    u_context_t_recover (! (!ctx)).payload #(Case_u_context_t_uds _);
+    context_t_recover (!ctx);
+    intro_owns_payload (!ctx)
+  );
+  return ctx;
+}
