test/engine/DPE.h
@@ -20,176 +20,27 @@ typedef struct _engine_record_t {
     ISARRAY(32) uint8_t *l0_image_auth_pubkey;        
 } engine_record_t;
 
-typedef struct {
-    uint32_t length;
-    //const char* data
-    //Vidush: Using uint8_t for now since const char* is not supported.
-    uint8_t *data;
-} fStar_Bytes_bytes;
-
-typedef struct _character_string_t_s{
-    uint32_t fst; 
-    fStar_Bytes_bytes snd;
-} character_string_t;
-
-typedef struct _octet_string_t_s{
-    uint32_t len; 
-    fStar_Bytes_bytes s;
-} octet_string_t;
-
-typedef struct _deviceIDCSR_ingredients_t_s
-{
-  int32_t ku;
-  int32_t version;
-  character_string_t s_common;
-  character_string_t s_org;
-  character_string_t s_country;
-}
-deviceIDCSR_ingredients_t;
-
-typedef struct aliasKeyCRT_ingredients_t_s
-{
-  int32_t version1;
-  octet_string_t serialNumber;
-  character_string_t i_common;
-  character_string_t i_org;
-  character_string_t i_country;
-  fStar_Bytes_bytes notBefore;
-  fStar_Bytes_bytes notAfter;
-  character_string_t s_common1;
-  character_string_t s_org1;
-  character_string_t s_country1;
-  int32_t ku1;
-  int32_t l0_version;
-} aliasKeyCRT_ingredients_t;
-
-typedef struct _l0_record_t_s
-{
-  uint8_t *fwid;
-  uint32_t deviceID_label_len;
-  uint8_t *deviceID_label;
-  uint32_t aliasKey_label_len;
-  uint8_t *aliasKey_label;
-  deviceIDCSR_ingredients_t deviceIDCSR_ingredients;
-  aliasKeyCRT_ingredients_t aliasKeyCRT_ingredients;
-} l0_record_t;
-
-typedef struct _l1_context_t_s
-{
-  uint8_t *deviceID_pub;
-  uint8_t *aliasKey_priv;
-  uint8_t *aliasKey_pub;
-  uint32_t deviceIDCSR_len;
-  uint8_t *deviceIDCSR;
-  uint32_t aliasKeyCRT_len;
-  uint8_t *aliasKeyCRT;
+typedef struct _l1_context_t {
+  ISARRAY(32) uint8_t *deviceID_pub;
+  ISARRAY(32) uint8_t *aliasKey_priv;
+  ISARRAY(32) uint8_t *aliasKey_pub;
+  size_t deviceIDCSR_len;
+  ISARRAY(deviceIDCSR_len) uint8_t *deviceIDCSR;
+  size_t aliasKeyCRT_len;
+  ISARRAY(aliasKeyCRT_len) uint8_t *aliasKeyCRT;
 } l1_context_t;
 
-#define Engine_context 0
-#define L0_context 1
-#define L1_context 2
+#define ENGINE_CONTEXT 0
+#define L0_CONTEXT 1
+#define L1_CONTEXT 2
 
-typedef uint8_t context_t_tags;
+typedef union _u_context_t {
+  ISARRAY(UDS_LEN) uint8_t *uds;
+  ISARRAY(DICE_DIGEST_LEN) uint8_t *cdi;
+  l1_context_t l1_context;
+} u_context_t;
 
-typedef struct _context_t_s
-{
-  context_t_tags tag;
-  union {
-    uint8_t *case_Engine_context;
-    uint8_t *case_L0_context;
-    l1_context_t case_L1_context;
-  } u;
+typedef struct _context_t {
+  uint8_t tag;
+  u_context_t payload;
 } context_t;
-
-#define Engine_record 0
-#define L0_record 1
-
-typedef uint8_t record_t_tags;
-
-typedef struct record_t_s
-{
-  record_t_tags tag;
-  union {
-    engine_record_t case_Engine_record;
-    l0_record_t case_L0_record;
-  } u;
-} record_t;
-
-typedef uint16_t dpe_sid_t;
-
-typedef context_t dpe_session_state__Available__payload;
-
-#define DPE_SessionStart 0
-#define DPE_Available 1
-#define DPE_InUse 2
-#define DPE_SessionClosed 3
-#define DPE_SessionError 4
-
-typedef uint8_t dpe_session_state_tags;
-
-typedef struct dpe_session_state_s
-{
-  dpe_session_state_tags tag;
-  dpe_session_state__Available__payload _0;
-} dpe_session_state;
-
-bool dpe_uu___is_SessionStart(dpe_session_state projectee);
-
-bool dpe_uu___is_Available(dpe_session_state projectee);
-
-bool dpe_uu___is_InUse(dpe_session_state projectee);
-
-bool dpe_uu___is_SessionClosed(dpe_session_state projectee);
-
-bool dpe_uu___is_SessionError(dpe_session_state projectee);
-
-#define Pulse_Lib_HashTable_Spec_Clean 0
-#define Pulse_Lib_HashTable_Spec_Zombie 1
-#define Pulse_Lib_HashTable_Spec_Used 2
-
-typedef uint8_t pulse_Lib_HashTable_Spec_cell__uint16_t_DPE_session_state_tags;
-
-typedef struct pulse_Lib_HashTable_Spec_cell__uint16_t_DPE_session_state_s
-{
-  pulse_Lib_HashTable_Spec_cell__uint16_t_DPE_session_state_tags tag;
-  uint16_t k;
-  dpe_session_state v;
-}
-pulse_Lib_HashTable_Spec_cell__uint16_t_DPE_session_state;
-
-typedef struct dpe_ht_t_s
-{
-  size_t sz;
-  //hashf : UInt16.t -> SizeT.t;
-  //size_t (*hashf)(uint16_t x0);
-  pulse_Lib_HashTable_Spec_cell__uint16_t_DPE_session_state *contents;
-} dpe_ht_t;
-
-typedef struct dpe_st_s
-{
-  uint16_t st_ctr;
-  dpe_ht_t st_tbl;
-} dpe_st;
-
-#define FStar_Pervasives_Native_None 0
-#define FStar_Pervasives_Native_Some 1
-
-typedef uint8_t fStar_Pervasives_Native_option__DPE_st_tags;
-
-typedef struct fStar_Pervasives_Native_option__uint16_t_s
-{
-  fStar_Pervasives_Native_option__DPE_st_tags tag;
-  uint16_t v;
-} fStar_Pervasives_Native_option__uint16_t;
-
-fStar_Pervasives_Native_option__uint16_t dpe_open_session(void);
-
-void dpe_initialize_context(uint16_t sid, uint8_t *uds);
-
-bool dpe_derive_child(uint16_t sid, record_t record);
-
-void dpe_close_session(uint16_t sid);
-
-uint32_t dpe_certify_key(uint16_t sid, uint8_t *pub_key, uint32_t crt_len, uint8_t *crt);
-
-void dpe_sign(uint16_t sid, uint8_t *signature, size_t msg_len, uint8_t *msg);
